@prefix : <#> .
@prefix dc: <http://purl.org/dc/elements/1.1/> .
@prefix dct: <http://purl.org/dc/terms/> .
@prefix ex: <http://example.org/> .
@prefix foaf: <http://xmlns.com/foaf/0.1/> .
@prefix marcrel: <http://id.loc.gov/vocabulary/relators/> .
@prefix oo: <http://purl.org/openorg/> .
@prefix rdf: <http://www.w3.org/1999/02/22-rdf-syntax-ns#> .
@prefix rdfs: <http://www.w3.org/2000/01/rdf-schema#> .
@prefix owl: <http://www.w3.org/2002/07/owl#> .
@prefix schema: <http://schema.org/> .
@prefix xsd: <http://www.w3.org/2001/XMLSchema#> .
@prefix gn: <http://www.geonames.org/ontology#> .

:ap
    a owl:Ontology , ex:ApplicationProfile ;
    dct:title "Application profile for OER world map prototype." ;
    dct:creator <http://lobid.org/person/ap> ;
    dct:created "2014-02-24" ;
    dc:rights "This application profile is available under the Creative Commons Public Domain Dedication (CC0)" ;
    dct:rights <http://creativecommons.org/publicdomain/zero/1.0/> .

:Organization
    a owl:Class ;
    rdfs:isDefinedBy :ap ;
    rdfs:subClassOf schema:Organization ,
    [ a owl:Restriction ;
        owl:onProperty :name ;
        owl:cardinality "1" ] ,
    [ a owl:Restriction ;
        owl:onProperty :alternateName ;
        owl:minCardinality "0" ] ,
    [ a owl:Restriction ;
        owl:onProperty :description ;
        owl:minCardinality "1" ] ,
    [ a owl:Restriction ;
        owl:onProperty :url ;
        owl:minCardinality "0" ] ,
    [ a owl:Restriction ;
        owl:onProperty :email ;
        owl:minCardinality "0" ] ,
    [ a owl:Restriction ;
        owl:onProperty :logo ;
        owl:minCardinality "0" ] ,
    [ a owl:Restriction ;
        owl:onProperty :address ;
        owl:minCardinality "0" ] ,
    [ a owl:Restriction ;
        owl:onProperty :geo ;
        owl:cardinality "1" ] ,
    [ a owl:Restriction ;
        owl:onProperty :sameAs ;
        owl:minCardinality "0" ] ,
    [ a owl:Restriction ;
        owl:onProperty :member ;
        owl:minCardinality "0" ] ,
    [ a owl:Restriction ;
        owl:onProperty :memberOf ;
        owl:minCardinality "0" ] ,
    [ a owl:Restriction ;
        owl:onProperty :providesService ;
        owl:minCardinality "0" ] .

:Person
    a owl:Class ;
    rdfs:isDefinedBy :ap ;
    rdfs:subClassOf schema:Person ,
    [ a owl:Restriction ;
        owl:onProperty :name ;
        owl:cardinality "1" ] ,
    [ a owl:Restriction ;
        owl:onProperty :alternateName ;
        owl:minCardinality "0" ] ,
    [ a owl:Restriction ;
        owl:onProperty :description ;
        owl:minCardinality "1" ] ,
    [ a owl:Restriction ;
        owl:onProperty :url ;
        owl:minCardinality "0" ] ,
    [ a owl:Restriction ;
        owl:onProperty :email ;
        owl:minCardinality "0" ] ,
    [ a owl:Restriction ;
        owl:onProperty :address ;
        owl:minCardinality "0" ] ,
    [ a owl:Restriction ;
        owl:onProperty :geo ;
        owl:minCardinality "0" ] ,
    [ a owl:Restriction ;
        owl:onProperty :sameAs ;
        owl:minCardinality "0" ] ,
    [ a owl:Restriction ;
        owl:onProperty :memberOf ;
        owl:minCardinality "0" ] .

:Service
    a owl:Class ;
    rdfs:isDefinedBy :ap ;
    rdfs:subClassOf schema:Service ,
    [ a owl:Restriction ;
        owl:onProperty :name ;
        owl:cardinality "1" ] ,
    [ a owl:Restriction ;
        owl:onProperty :alternateName ;
        owl:minCardinality "0" ] ,
    [ a owl:Restriction ;
        owl:onProperty :description ;
        owl:minCardinality "1" ] ,
    [ a owl:Restriction ;
        owl:onProperty :url ;
        owl:minCardinality "0" ] ,
    [ a owl:Restriction ;
        owl:onProperty :email ;
        owl:minCardinality "0" ] ,
    [ a owl:Restriction ;
        owl:onProperty :logo ;
        owl:minCardinality "0" ] ,
    [ a owl:Restriction ;
        owl:onProperty :contact ;
        owl:minCardinality "0" ] ,
    [ a owl:Restriction ;
        owl:onProperty :license ;
        owl:minCardinality "1" ] ,
    [ a owl:Restriction ;
        owl:onProperty :sameAs ;
        owl:minCardinality "0" ] ,
    [ a owl:Restriction ;
        owl:onProperty :provider ;
        owl:minCardinality "0" ] .

:Project
    a owl:Class ;
    rdfs:isDefinedBy :ap ;
    rdfs:subClassOf foaf:Project ,
    [ a owl:Restriction ;
        owl:onProperty :name ;
        owl:cardinality "1" ] ,
    [ a owl:Restriction ;
        owl:onProperty :alternateName ;
        owl:minCardinality "0" ] ,
    [ a owl:Restriction ;
        owl:onProperty :description ;
        owl:minCardinality "1" ] ,
    [ a owl:Restriction ;
        owl:onProperty :url ;
        owl:minCardinality "0" ] ,
    [ a owl:Restriction ;
        owl:onProperty :email ;
        owl:minCardinality "0" ] ,
    [ a owl:Restriction ;
        owl:onProperty :logo ;
        owl:minCardinality "0" ] ,
    [ a owl:Restriction ;
        owl:onProperty :contact ;
        owl:minCardinality "0" ] ,
    [ a owl:Restriction ;
        owl:onProperty :sameAs ;
        owl:minCardinality "0" ] ,
    [ a owl:Restriction ;
        owl:onProperty :member ;
        owl:allValuesFrom :Person ;
        owl:minCardinality "0" ] .

:PostalAddress
    a owl:Class ;
    rdfs:isDefinedBy :ap ;
    rdfs:subClassOf schema:PostalAddress ,
    [ a owl:Restriction ;
        owl:onProperty :streetAddress ;
        owl:cardinality "1" ] ,
    [ a owl:Restriction ;
        owl:onProperty :postalCode ;
        owl:cardinality "1" ] ,
    [ a owl:Restriction ;
        owl:onProperty :addressLocality ;
        owl:cardinality "1" ] ,
    [ a owl:Restriction ;
        owl:onProperty :addressCountry ;
        owl:cardinality "1" ] .

:GeoCoordinates
    a owl:Class ;
    rdfs:isDefinedBy :ap ;
    rdfs:subClassOf schema:GeoCoordinates ,
    [ a owl:Restriction ;
        owl:onProperty :latitude ;
        owl:cardinality "1" ] ,
    [ a owl:Restriction ;
        owl:onProperty :longitude ;
        owl:cardinality "1" ] .

:Image
    a owl:Class ;
    rdfs:isDefinedBy :ap ;
    rdfs:subClassOf foaf:Image .

:Locality
    a owl:Class ;
    rdfs:isDefinedBy :ap ;
    rdfs:subClassOf gn:Feature ,
    [ a owl:Restriction ;
        owl:onProperty gn:featureClass ;
        owl:hasValue gn:P ] ,
    [ a owl:Restriction ;
        owl:onProperty :featureName ;
        owl:cardinality "0" ] .

:Country
    a owl:Class ;
    rdfs:isDefinedBy :ap ;
    rdfs:subClassOf gn:Feature ,
    [ a owl:Restriction ;
        owl:onProperty gn:featureClass ;
        owl:hasValue gn:A ] ,
    [ a owl:Restriction ;
        owl:onProperty :featureName ;
        owl:cardinality "0" ] .

:featureName
    a owl:DatatypeProperty ;
    rdfs:comment "In the context of this application profile the property gn:name is used to indicate the name of a geonames feature."@en ;
    rdfs:subPropertyOf gn:name ;
    rdfs:isDefinedBy :ap ;
    rdfs:label "Name"@en ;
    rdfs:label "Name"@de ;
    rdfs:range rdfs:Literal .

<http://api.geonames.org/search>
    a ex:endpoint ;
    ex:queryParam "q" ;
    ex:offsetParam "startRow" ;
    ex:limitParam "maxRows" ;
    ex:additionalParam "username=literarymachine" , "type=rdf";
    ex:resultFormat "application/rdf+xml" ;
    ex:supplies :Locality , :Country .

<http://api.lobid.org/oer>
    a ex:endpoint ;
    ex:queryParam "q" ;
    ex:typeParam "t" ;
    ex:offsetParam "from" ;
    ex:limitParam "size" ;
    ex:resultFormat "application/rdf+xml" ;
    ex:supplies :Organization , :Service , :Person , :Project .

:type
    a owl:ObjectProperty ;
    rdfs:comment "In the context of this application profile the property rdf:type is used to indicate the type of a resource (person, organization, project, or service)."@en ;
    rdfs:subPropertyOf rdf:type ;
    rdfs:isDefinedBy :ap ;
    rdfs:label "Type"@en ;
    rdfs:label "Typ"@de ;
    rdfs:range [
      a owl:Class ;
      owl:oneOf ( :Organization :Service :Person :Project )
    ] .

:logo
    a owl:ObjectProperty ;
    rdfs:comment "In the context of this application profile the property schema:logo is used to link to a logo of an organization, a project, or a service."@en ;
    rdfs:subPropertyOf schema:logo ;
    rdfs:isDefinedBy :ap ;
    rdfs:label "Logo"@en ;
    rdfs:label "Logo"@de ;
    rdfs:range :Image .

:name
    a owl:DatatypeProperty ;
    rdfs:comment "In the context of this application profile the property schema:name is used to indicate the name of a person, organization, project, or service."@en ;
    rdfs:subPropertyOf schema:name ;
    rdfs:isDefinedBy :ap ;
    rdfs:label "Name"@en ;
    rdfs:label "Name"@de ;
    rdfs:range rdfs:Literal .

:alternateName
    a owl:DatatypeProperty ;
    rdfs:comment "In the context of this application profile the property schema:alternateName is used to indicate the alternate name (nick name, abbreviation etc.) of a person, organization, project, or service."@en ;
    rdfs:subPropertyOf schema:alternateName ;
    rdfs:isDefinedBy :ap ;
    rdfs:label "Alternate Name"@en ;
    rdfs:label "Alternativer Name"@de ;
    rdfs:range rdfs:Literal .

:description
    a owl:DatatypeProperty ;
    rdfs:comment "In the context of this application profile the property schema:description is used to give a description of a person, organization, project, or service."@en ;
    rdfs:subPropertyOf schema:description ;
    rdfs:isDefinedBy :ap ;
    rdfs:label "Description"@en ;
    rdfs:label "Beschreibung"@de ;
    rdfs:range rdfs:Literal .

:url
    a owl:DatatypeProperty ;
    rdfs:comment "In the context of this application profile the property schema:url is used to link to a homepage of a person, organization, project, or service."@en ;
    rdfs:subPropertyOf schema:url ;
    rdfs:isDefinedBy :ap ;
    rdfs:label "Website"@en ;
    rdfs:label "Webseite"@de ;
    rdfs:range schema:WebPage .

:email
    a owl:DatatypeProperty ;
    rdfs:comment "In the context of this application profile the property schema:email is used to indicate the email address of a person, organization, project, or service. The literal should conform to this regular expression: [A-Z0-9._%+-]+@[A-Z0-9.-]+.[A-Z]{2,4}"@en ;
    rdfs:subPropertyOf schema:email ;
    rdfs:isDefinedBy :ap ;
    rdfs:label "Email"@en ;
    rdfs:label "E-Mail"@de ;
    rdfs:range [
      a rdfs:Datatype ;
      owl:onDatatype xsd:string ;
      owl:withRestrictions (
        [
            xsd:pattern "[A-Z0-9._%+-]+@[A-Z0-9.-]+.[A-Z]{2,4}"
        ]
      )
    ] .

:contact
    a owl:ObjectProperty ;
    rdfs:comment "In the context of this application profile the property oo:contact is used to link a project or service to a contact person within the OER map data."@en ;
    rdfs:subPropertyOf oo:contact ;
    rdfs:isDefinedBy :ap ;
    rdfs:label "Contact Person"@en ;
    rdfs:label "Kontaktperson"@de ;
    rdfs:range :Person .

:address
    a owl:ObjectProperty ;
    rdfs:comment "In the context of this application profile the property schema:address is used to link to a blank node with address details of a person or an organization."@en ;
    rdfs:subPropertyOf schema:address ;
    rdfs:isDefinedBy :ap ;
    rdfs:label "Address"@en ;
    rdfs:label "Adresse"@de ;
    rdfs:range :PostalAddress .

:streetAddress
    a owl:DatatypeProperty ;
    rdfs:comment "In the context of this application profile the property schema:streetAddress is used to indicate the street address of a schema:PostalAddress."@en ;
    rdfs:subPropertyOf schema:streetAddress ;
    rdfs:isDefinedBy :ap ;
    rdfs:label "Street Address"@en ;
    rdfs:label "Straße und Hausnummer"@de ;
    rdfs:domain :PostalAddress ;
    rdfs:range rdfs:Literal .

:postalCode
    a owl:DatatypeProperty ;
    rdfs:comment "In the context of this application profile the property schema:postalCode is used to indicate the postal code of a schema:PostalAddress."@en ;
    rdfs:subPropertyOf schema:postalCode ;
    rdfs:isDefinedBy :ap ;
    rdfs:label "Postal Code"@en ;
    rdfs:label "Postleitzahl"@de ;
    rdfs:domain :PostalAddress ;
    rdfs:range rdfs:Literal .

:addressLocality
    a owl:ObjectProperty ;
    rdfs:comment "In the context of this application profile the property schema:addressLocality is used to indicate the locality of a schema:PostalAddress using the respective GeoNames URI."@en ;
    rdfs:subPropertyOf schema:addressLocality ;
    rdfs:isDefinedBy :ap ;
    rdfs:label "Locality"@en ;
    rdfs:label "Ort"@de ;
    rdfs:domain :PostalAddress ;
    rdfs:range :Locality .

:addressCountry
    a owl:ObjectProperty ;
    rdfs:comment "In the context of this application profile the property schema:addressCountry is used to indicate the country of a schema:PostalAddress using the respective GeoNames URI."@en ;
    rdfs:subPropertyOf schema:addressCountry ;
    rdfs:isDefinedBy :ap ;
    rdfs:label "Country"@en ;
    rdfs:label "Ort"@de ;
    rdfs:domain :PostalAddress ;
    rdfs:range :Country .

:license
    a owl:ObjectProperty ;
    rdfs:comment "In the context of this application profile the property dct:license is used to link a service to the license the service's contents are licensed under."@en ;
    rdfs:subPropertyOf dct:license ;
    rdfs:isDefinedBy :ap ;
    rdfs:label "License"@en ;
    rdfs:label "Lizenz"@de .

:geo
    a owl:ObjectProperty ;
    rdfs:comment "In the context of this application profile the property schema:geo is used to link an organization to its schema:GeoCoordinates."@en ;
    rdfs:subPropertyOf schema:geo ;
    rdfs:isDefinedBy :ap ;
    rdfs:label "Geo Coordinates"@en ;
    rdfs:label "Geokoordinaten"@de ;
    rdfs:range :GeoCoordinates .

:latitude
    a owl:DatatypeProperty ;
    rdfs:comment "In the context of this application profile the property schema:latitude is used to indicate the latitude of schema:GeoCoordinates. Values should conform to this regular expression: ^(-?[0-9]+(.[0-9]+)?), *(-?[0-9]+(.[0-9]+)?)$ ."@en ;
    rdfs:subPropertyOf schema:latitude ;
    rdfs:isDefinedBy :ap ;
    rdfs:label "Latitude"@en ;
    rdfs:label "Geographische Breite"@de ;
    rdfs:range [
      a rdfs:Datatype ;
      owl:onDatatype xsd:string ;
      owl:withRestrictions (
        [
            xsd:pattern "^(-?[0-9]+(.[0-9]+)?), *(-?[0-9]+(.[0-9]+)?)$"
        ]
      )
    ] .

:longitude
    a owl:DatatypeProperty ;
    rdfs:comment "In the context of this application profile the property schema:longitude is used to indicate the longitude of schema:GeoCoordinates. Values should conform to this regular expression: ^(-?[0-9]+(.[0-9]+)?), *(-?[0-9]+(.[0-9]+)?)$ ."@en ;
    rdfs:subPropertyOf schema:longitude ;
    rdfs:isDefinedBy :ap ;
    rdfs:label "Longitude"@en ;
    rdfs:label "Geographische Länge"@de ;
    rdfs:range [
      a rdfs:Datatype ;
      owl:onDatatype xsd:string ;
      owl:withRestrictions (
        [
            xsd:pattern "^(-?[0-9]+(.[0-9]+)?), *(-?[0-9]+(.[0-9]+)?)$"
        ]
      )
    ] .

:sameAs
    a owl:ObjectProperty ;
    rdfs:comment "In the context of this application profile the property schema:sameAs is used to link an organizatin, a person, a service or a project to other URIs for them."@en ;
    rdfs:subPropertyOf schema:sameAs ;
    rdfs:isDefinedBy :ap ;
    rdfs:label "Same as"@en ;
    rdfs:label "Identische Ressource"@de .

:member
    a owl:ObjectProperty ;
    rdfs:comment "In the context of this application profile the property schema:member is used to link an organization or project to persons or other organizations that are members of the organization/project."@en ;
    rdfs:subPropertyOf schema:member ;
    rdfs:isDefinedBy :ap ;
    rdfs:label "Members"@en ;
    rdfs:label "Mitglieder"@de ;
    rdfs:range [
      a owl:Class ;
      owl:oneOf ( :Organization :Person )
    ] .

:memberOf
    a owl:ObjectProperty ;
    rdfs:comment "In the context of this application profile the property schema:memberOf is used to link an organization or a person to organizations or projects they are members of."@en ;
    rdfs:subPropertyOf schema:memberOf ;
    rdfs:isDefinedBy :ap ;
    rdfs:label "Member of"@en ;
    rdfs:label "Mitglied von"@de ;
    rdfs:range [
      a owl:Class ;
      owl:oneOf ( :Organization :Project )
    ] .

:providesService
    a owl:ObjectProperty ;
    rdfs:comment "In the context of this application profile the property schema:providesService is used to link an organization to an OER service it provides."@en ;
    rdfs:subPropertyOf schema:providesService ;
    rdfs:isDefinedBy :ap ;
    rdfs:label "OER services by the organization"@en ;
    rdfs:label "OER-Angebote der Organisation"@de ;
    rdfs:range :Service .

:provider
    a owl:ObjectProperty ;
    rdfs:comment "In the context of this application profile the property schema:provider is used to link an OER service to an organization that provides the service."@en ;
    rdfs:subPropertyOf schema:provider ;
    rdfs:isDefinedBy :ap ;
    rdfs:label "Provider"@en ;
    rdfs:label "Anbieter"@de ;
    rdfs:range :Organization .

:funder
    a owl:ObjectProperty ;
    rdfs:comment "In the context of this application profile the property marcrel:fnd is used to link a project to an organization that funds the project."@en ;
    rdfs:subPropertyOf marcrel:fnd ;
    rdfs:isDefinedBy :ap ;
    rdfs:label "Funding Organization"@en ;
    rdfs:label "Gefördert von"@de ;
    rdfs:range :Organization .
